@prefix : <https://purl.org/ontocosmetic#> .
@prefix owl: <http://www.w3.org/2002/07/owl#> .
@prefix rdf: <http://www.w3.org/1999/02/22-rdf-syntax-ns#> .
@prefix xml: <http://www.w3.org/XML/1998/namespace> .
@prefix xsd: <http://www.w3.org/2001/XMLSchema#> .
@prefix rdfs: <http://www.w3.org/2000/01/rdf-schema#> .
@base <https://purl.org/ontocosmetic#> .

<https://purl.org/ontocosmetic> rdf:type owl:Ontology ;
                                 owl:versionIRI <https://purl.org/ontocosmetic/4.0> ;
                                 <http://purl.org/dc/elements/1.1/contributor> "Juliana Serna Rodas" ;
                                 <http://purl.org/dc/elements/1.1/creator> "Alex Gabriel" ;
                                 <http://purl.org/dc/elements/1.1/description> "An ontology that describes chemical formulation in the perspective to assist the design process of cosmetic product."@en ;
                                 <http://purl.org/dc/elements/1.1/title> "Onto Cosmetic"@en ;
                                 owl:priorVersion "3.0"@en ;
                                 owl:versionInfo "4.0"@en .

#################################################################
#    Annotation properties
#################################################################

###  http://purl.org/dc/elements/1.1/contributor
<http://purl.org/dc/elements/1.1/contributor> rdf:type owl:AnnotationProperty .


###  http://purl.org/dc/elements/1.1/creator
<http://purl.org/dc/elements/1.1/creator> rdf:type owl:AnnotationProperty .


###  http://purl.org/dc/elements/1.1/description
<http://purl.org/dc/elements/1.1/description> rdf:type owl:AnnotationProperty .


###  http://purl.org/dc/elements/1.1/publisher
<http://purl.org/dc/elements/1.1/publisher> rdf:type owl:AnnotationProperty .


###  http://purl.org/dc/elements/1.1/title
<http://purl.org/dc/elements/1.1/title> rdf:type owl:AnnotationProperty .


###  http://swrl.stanford.edu/ontologies/3.3/swrla.owl#isRuleEnabled
<http://swrl.stanford.edu/ontologies/3.3/swrla.owl#isRuleEnabled> rdf:type owl:AnnotationProperty .


#################################################################
#    Object Properties
#################################################################

###  https://purl.org/ontocosmetic#definesStateOf
:definesStateOf rdf:type owl:ObjectProperty ;
                rdfs:domain :PropertyState ;
                rdfs:range :Property ;
                rdfs:comment "Relationship between qualitative state of substance property and the property."@en ;
                rdfs:label "defines state of"@en .


###  https://purl.org/ontocosmetic#hasAfterfeeling
:hasAfterfeeling rdf:type owl:ObjectProperty ;
                 rdfs:domain :Emollient ;
                 rdfs:range :AfterfeelingState ;
                 rdfs:comment "Give one or several afterfeeling properties to an ingredient of type emollient."@en ;
                 rdfs:label "has afterfeeling"@en .


###  https://purl.org/ontocosmetic#hasChemicalNature
:hasChemicalNature rdf:type owl:ObjectProperty ,
                            owl:FunctionalProperty ;
                   rdfs:domain :Ingredient ;
                   rdfs:range :Chemical_nature ;
                   rdfs:comment "Give the chemical nature of an ingredient."@en ;
                   rdfs:label "has chemical nature"@en .


###  https://purl.org/ontocosmetic#hasDosage
:hasDosage rdf:type owl:ObjectProperty ;
           rdfs:domain :Formulation ;
           rdfs:range :Dosage ;
           rdfs:comment "Give the dosages that composes a formulation."@en ;
           rdfs:label "has dosage"@en .


###  https://purl.org/ontocosmetic#hasEmollience
:hasEmollience rdf:type owl:ObjectProperty ;
               rdfs:domain :Emollient ;
               rdfs:range :EmollienceState ;
               rdfs:comment "Give the level of emollience of an ingredient of type emollient."@en ;
               rdfs:label "has emollience level"@en .


###  https://purl.org/ontocosmetic#hasHeuristicIngProp
:hasHeuristicIngProp rdf:type owl:ObjectProperty ;
                     rdfs:domain :Heuristic ;
                     rdfs:range :Property ;
                     rdfs:comment "Associate an heuristic to the ingredient property that is involved in the rule."@en ;
                     rdfs:label "is affected by ingredient property"@en .


###  https://purl.org/ontocosmetic#hasHeuristicIngType
:hasHeuristicIngType rdf:type owl:ObjectProperty ;
                     rdfs:domain :Heuristic ;
                     rdfs:range :ChemicalFamily ;
                     rdfs:comment "Define which ingredient type is concerned by the heuristic."@en ;
                     rdfs:label "involves ingredient type"@en .


###  https://purl.org/ontocosmetic#hasHeuristicProcessOutcome
:hasHeuristicProcessOutcome rdf:type owl:ObjectProperty ;
                            rdfs:domain :Heuristic ;
                            rdfs:range :DropletSizeState ;
                            rdfs:comment "Associate a heuristic to the structure property of the formulation final product  that is involved in the rule."@en ;
                            rdfs:label "has structural property"@en .


###  https://purl.org/ontocosmetic#hasHeuristicProcessProp
:hasHeuristicProcessProp rdf:type owl:ObjectProperty ;
                         rdfs:domain :Heuristic ;
                         rdfs:range :UnitOperation ;
                         rdfs:comment "Associate an heuristic to the process used to do the formulation final product. This process will have an impact on the product structure or properties."@en ;
                         rdfs:label "is produced through"@en .


###  https://purl.org/ontocosmetic#hasHeuristicProdProp
:hasHeuristicProdProp rdf:type owl:ObjectProperty ;
                      rdfs:domain :Heuristic ;
                      rdfs:range :Property ;
                      rdfs:comment "Associate an heuristic to a product property. The rule has an impact on the properties of the final product formulated."@en .


###  https://purl.org/ontocosmetic#hasHeuristicProductPropertyState
:hasHeuristicProductPropertyState rdf:type owl:ObjectProperty ;
                                  rdfs:domain :Heuristic ;
                                  rdfs:range :PropertyState ;
                                  rdfs:comment "Define the state that is given to the property when the heuristic is verified."@en .


###  https://purl.org/ontocosmetic#hasIngredient
:hasIngredient rdf:type owl:ObjectProperty ;
               rdfs:domain :Formulation ;
               rdfs:range :Ingredient ;
               rdfs:comment "Relationship that defines the ingredients that are used in a formulation."@en ;
               rdfs:label "has ingredient"@en .


###  https://purl.org/ontocosmetic#hasIngredientPropertyState
:hasIngredientPropertyState rdf:type owl:ObjectProperty ;
                            rdfs:domain :Heuristic ;
                            rdfs:range :PropertyState ;
                            rdfs:comment "Defines a relation between an heuristic and a specific state of a property. It defines the property state that could trigger the heuristic."@en ;
                            rdfs:label "has ingredient property state"@en .


###  https://purl.org/ontocosmetic#hasIonicClass
:hasIonicClass rdf:type owl:ObjectProperty ,
                        owl:FunctionalProperty ;
               rdfs:domain :Surfactant ;
               rdfs:range :IonicState ;
               rdfs:comment "Define the ionic nature of an ingredient."@en .


###  https://purl.org/ontocosmetic#hasOrigin
:hasOrigin rdf:type owl:ObjectProperty ;
           rdfs:domain :Ingredient ;
           rdfs:range :Origin ;
           rdfs:comment "Provide the origin of an ingredient"@en ;
           rdfs:label "has origin"@en .


###  https://purl.org/ontocosmetic#hasPhase
:hasPhase rdf:type owl:ObjectProperty ;
          rdfs:domain :Ingredient ;
          rdfs:range :PhaseState ;
          rdfs:comment "it define which phase the ingredient is soluble in."@en .


###  https://purl.org/ontocosmetic#hasProcess
:hasProcess rdf:type owl:ObjectProperty ;
            rdfs:domain :Formulation ;
            rdfs:range :Process ;
            rdfs:comment "Processing done on the ingredient of the formulation."@en .


###  https://purl.org/ontocosmetic#hasProductDropletSize
:hasProductDropletSize rdf:type owl:ObjectProperty ;
                       rdfs:domain :Formulation ;
                       rdfs:range :DropletSizeState ;
                       rdfs:comment "Provides the size of the droplet of the final product of a formulation. This droplet will depends on process."@en .


###  https://purl.org/ontocosmetic#hasProductOiliness
:hasProductOiliness rdf:type owl:ObjectProperty ;
                    rdfs:domain :Formulation ;
                    rdfs:range :Oiliness ;
                    rdfs:comment "Define the oiliness of formulated product."@en .


###  https://purl.org/ontocosmetic#hasProductStability
:hasProductStability rdf:type owl:ObjectProperty ;
                     rdfs:domain :Formulation ;
                     rdfs:range :StabilityState ;
                     rdfs:comment "Define the stability of a formulation final product."@en .


###  https://purl.org/ontocosmetic#hasProductViscosity
:hasProductViscosity rdf:type owl:ObjectProperty ;
                     rdfs:domain :Formulation ;
                     rdfs:range :ViscosityState ;
                     rdfs:comment "Provides the viscosity of the formulation final product."@en .


###  https://purl.org/ontocosmetic#hasQualitativeValue
:hasQualitativeValue rdf:type owl:ObjectProperty ;
                     rdfs:domain :Property ;
                     rdfs:range :PropertyState ;
                     rdfs:comment "Relationship that link a property to the qualitative value that are associated to the property."@en ;
                     rdfs:label "has qualitative value"@en .


###  https://purl.org/ontocosmetic#hasSpreading
:hasSpreading rdf:type owl:ObjectProperty ;
              rdfs:domain :Emollient ;
              rdfs:range :SpreadingState ;
              rdfs:comment "Defines the spreading property of an emollient."@en .


###  https://purl.org/ontocosmetic#hasState
:hasState rdf:type owl:ObjectProperty ;
          rdfs:domain :Substance ;
          rdfs:range :StateOfMatter .


###  https://purl.org/ontocosmetic#hasTexture
:hasTexture rdf:type owl:ObjectProperty ;
            rdfs:domain :Surfactant ;
            rdfs:range :TextureState ;
            rdfs:comment "Provides the texture that can be expected from a given surfactant."@en .


###  https://purl.org/ontocosmetic#isCommercializedAs
:isCommercializedAs rdf:type owl:ObjectProperty ;
                    rdfs:domain :Formulation ;
                    rdfs:range :Product ;
                    rdfs:comment "Relate a formulation with a product that is commercialized or will be."@en ;
                    rdfs:label "is commercialized as"@en .


###  https://purl.org/ontocosmetic#isPropertyOf
:isPropertyOf rdf:type owl:ObjectProperty ;
              rdfs:domain :Property ;
              rdfs:range :ChemicalFamily ;
              rdfs:comment "Define the type of substance (chemical nature) that is concerned by the property."@en ;
              rdfs:label "is property of"@en .


###  https://purl.org/ontocosmetic#isQuantifying
:isQuantifying rdf:type owl:ObjectProperty ;
               rdfs:domain :Dosage ;
               rdfs:range :Ingredient ;
               rdfs:comment "Give the ingredient of a dosage."@en ;
               rdfs:label "is quantifying"@en .


###  https://purl.org/ontocosmetic#isValidatedBy
:isValidatedBy rdf:type owl:ObjectProperty ;
               rdfs:domain :Formulation ;
               rdfs:range :Heuristic ;
               rdfs:comment "Defines that a formulation validate a given heuristic."@en .


#################################################################
#    Data properties
#################################################################

###  https://purl.org/ontocosmetic#hasCalculatedHLB
:hasCalculatedHLB rdf:type owl:DatatypeProperty ;
                  rdfs:domain :Formulation ;
                  rdfs:range xsd:float ;
                  rdfs:comment "the final HLB of the surfactant mixture that compose the formulation"@en .


###  https://purl.org/ontocosmetic#hasEquivalentHLB
:hasEquivalentHLB rdf:type owl:DatatypeProperty .


###  https://purl.org/ontocosmetic#hasHLB
:hasHLB rdf:type owl:DatatypeProperty ;
        rdfs:domain :Surfactant ;
        rdfs:comment "the HLB that a surfactant can have"@en .


###  https://purl.org/ontocosmetic#hasHeuristicDescription
:hasHeuristicDescription rdf:type owl:DatatypeProperty ;
                         rdfs:domain :Heuristic ;
                         rdfs:comment "Data properties that provides a description of the heuristic."@en .


###  https://purl.org/ontocosmetic#hasHeuristicHighThreshold
:hasHeuristicHighThreshold rdf:type owl:DatatypeProperty ;
                           rdfs:domain :Heuristic ;
                           rdfs:range xsd:float ;
                           rdfs:comment "High threshold in percentage for an heuristique."@en .


###  https://purl.org/ontocosmetic#hasHeuristicLowThreshold
:hasHeuristicLowThreshold rdf:type owl:DatatypeProperty ;
                          rdfs:domain :Heuristic ;
                          rdfs:range xsd:float ;
                          rdfs:comment "Low threshold in percentage for an heuristique."@en .


###  https://purl.org/ontocosmetic#hasHeuristicSource
:hasHeuristicSource rdf:type owl:DatatypeProperty ;
                    rdfs:domain :Heuristic ;
                    rdfs:comment "Provides the source of the heuristic (from literature or experience)"@en .


###  https://purl.org/ontocosmetic#hasINCIcode
:hasINCIcode rdf:type owl:DatatypeProperty ;
             rdfs:domain :Ingredient ;
             rdfs:range xsd:string ;
             rdfs:comment "the INCI code that a ingredient can have."@en .


###  https://purl.org/ontocosmetic#hasNbSurfactantIng
:hasNbSurfactantIng rdf:type owl:DatatypeProperty ;
                    rdfs:domain :Formulation ;
                    rdfs:range xsd:int ;
                    rdfs:comment "Define the number of surfactants inside a given formulation."@en .


###  https://purl.org/ontocosmetic#hasPricePerKilogram
:hasPricePerKilogram rdf:type owl:DatatypeProperty ;
                     rdfs:domain :Ingredient ;
                     rdfs:range xsd:float ;
                     rdfs:comment "Price per kilogram of an ingredient"@en .


###  https://purl.org/ontocosmetic#hasProductOilyPhase
:hasProductOilyPhase rdf:type owl:DatatypeProperty ;
                     rdfs:domain :Formulation ;
                     rdfs:range xsd:float ;
                     rdfs:comment "Percentage of the formulated product that represent oily ingrdient."@en .


###  https://purl.org/ontocosmetic#hasQuantity
:hasQuantity rdf:type owl:DatatypeProperty ,
                      owl:FunctionalProperty ;
             rdfs:domain :Dosage ;
             rdfs:range xsd:float ;
             rdfs:comment "the quantity of ingredient that compose the dosage. This quantity is in percentage of volume of the formulation."@en .


###  https://purl.org/ontocosmetic#hasRequiredHLB
:hasRequiredHLB rdf:type owl:DatatypeProperty ;
                rdfs:domain :Emollient ;
                rdfs:comment "the RHLB that an emollient can have."@en .


###  https://purl.org/ontocosmetic#hasTotalOilyPhase
:hasTotalOilyPhase rdf:type owl:DatatypeProperty ;
                   rdfs:domain :Formulation ;
                   rdfs:range xsd:float .


###  https://purl.org/ontocosmetic#hasTotalSurfactantQuantity
:hasTotalSurfactantQuantity rdf:type owl:DatatypeProperty ,
                                     owl:FunctionalProperty ;
                            rdfs:domain :Formulation ;
                            rdfs:range xsd:float ;
                            rdfs:comment "The total quantity of surfactant that a formulation has. This quantity is in percentage of volume."@en .


###  https://purl.org/ontocosmetic#hasTotalThickenerQuantity
:hasTotalThickenerQuantity rdf:type owl:DatatypeProperty ;
                           rdfs:domain :Formulation ;
                           rdfs:range xsd:float ;
                           rdfs:comment "The total quantity of thickener that a formulation has. This quantity is in percentage of volume."@en .


#################################################################
#    Classes
#################################################################

###  https://purl.org/ontocosmetic#AbsorptionRateState
:AbsorptionRateState rdf:type owl:Class ;
                     rdfs:subClassOf :FormulationPropertyState ;
                     rdfs:comment "Describe the capacity of the formulation product to be absopt by a skin."@en ;
                     rdfs:label "After Feel - Absorption Rate"@en .


###  https://purl.org/ontocosmetic#Active
:Active rdf:type owl:Class ;
        rdfs:subClassOf :Ingredient ;
        rdfs:comment "Ingredients that perform an specific function on customer skin. [cosmetic sector definition]. It is a chemical that helps with the main function of the cosmetic product."@en ;
        rdfs:label "Active"@en .


###  https://purl.org/ontocosmetic#Aerosol
:Aerosol rdf:type owl:Class ;
         rdfs:subClassOf :Colloid ;
         rdfs:comment "solid or liquid particles in a gas"@en .


###  https://purl.org/ontocosmetic#AfterfeelingState
:AfterfeelingState rdf:type owl:Class ;
                   rdfs:subClassOf :IngredientPropertyState ;
                   rdfs:comment "Ingredients have the property to influence the afterfeel of the formulated product."@en .


###  https://purl.org/ontocosmetic#AgitationState
:AgitationState rdf:type owl:Class ;
                rdfs:subClassOf :ProcessState ;
                rdfs:label "Agitatione state"@en ,
                           "Define the qualitative that the agitation process can have."@en .


###  https://purl.org/ontocosmetic#AmphotericSurfactant
:AmphotericSurfactant rdf:type owl:Class ;
                      rdfs:subClassOf :IonicSurfactant .


###  https://purl.org/ontocosmetic#AnionicSurfactant
:AnionicSurfactant rdf:type owl:Class ;
                   rdfs:subClassOf :IonicSurfactant .


###  https://purl.org/ontocosmetic#AnionicThickener
:AnionicThickener rdf:type owl:Class ;
                  rdfs:subClassOf :IonicThickener ;
                  rdfs:label "Anionic thickener"@en .


###  https://purl.org/ontocosmetic#Antioxidant
:Antioxidant rdf:type owl:Class ;
             rdfs:subClassOf :Active ;
             rdfs:comment "Chemicals that interrupt oxidation reactions and prevent the effects of oxygen radicals (e.g. peroxides) both processes known to damage the integrity and function of various natural substances. Antioxidants are useful in two ways: On the one hand they prevent degradation of natural ingredients (proteins, sugars, lipids) in the cosmetic product. On the other hand antioxidants protect the skin cells from being damaged and slow down the aging process. Antioxidants have been shown to boost the skin's radiance, minimize age spots, sun spots, and fine lines."@en .


###  https://purl.org/ontocosmetic#AqueousThickeners
:AqueousThickeners rdf:type owl:Class ;
                   rdfs:subClassOf :Thickener ;
                   rdfs:label "Aqueous Thickeners"@en .


###  https://purl.org/ontocosmetic#CationicSurfactant
:CationicSurfactant rdf:type owl:Class ;
                    rdfs:subClassOf :IonicSurfactant .


###  https://purl.org/ontocosmetic#CationicThickener
:CationicThickener rdf:type owl:Class ;
                   rdfs:subClassOf :IonicThickener ;
                   rdfs:label "Cationic thickener"@en .


###  https://purl.org/ontocosmetic#ChelatingAgent
:ChelatingAgent rdf:type owl:Class ;
                rdfs:subClassOf :OtherIngredient ;
                rdfs:comment "A substance that reacts with metal ions to form stable, water-soluble metal. They are used in liquid soap and body wash to prevent fragrance and color degradation and for their synergistic effect with antimicrobials. The process of chelation stabilizes metal ions by preventing them from chemically reacting with any other substances."@en ;
                rdfs:label "Chelating agent"@en .


###  https://purl.org/ontocosmetic#ChemicalFamily
:ChemicalFamily rdf:type owl:Class ;
                rdfs:subClassOf :PropertyState .


###  https://purl.org/ontocosmetic#Chemical_nature
:Chemical_nature rdf:type owl:Class ;
                 rdfs:subClassOf :PropertyState ;
                 rdfs:comment "Classification that a substance can have"@en ;
                 rdfs:label "Chemical nature"@en .


###  https://purl.org/ontocosmetic#Colloid
:Colloid rdf:type owl:Class ;
         rdfs:subClassOf :HeterogenousMixture ;
         rdfs:comment "It is a heterogeneous mixture in which a substance with a microscopic structure of disperse insoluble particles (disperse phase) is suspended in another substance (continuous phase). It can exist naturally, or it can be technically formulated, and in that case, it can also be named as a Formulation."@en ;
         rdfs:seeAlso "colloidal system"@en .


###  https://purl.org/ontocosmetic#Dosage
:Dosage rdf:type owl:Class ;
        rdfs:comment "Dosages are the combination of an ingredient and a quantity. It constitute a part of a formulation."@en ;
        rdfs:label "Dosage"@en .


###  https://purl.org/ontocosmetic#DropletSizeState
:DropletSizeState rdf:type owl:Class ;
                  rdfs:subClassOf :StructurePropertyState ;
                  rdfs:label "Droplet size state"@en .


###  https://purl.org/ontocosmetic#EmollienceState
:EmollienceState rdf:type owl:Class ;
                 rdfs:subClassOf :PropertyState .


###  https://purl.org/ontocosmetic#Emollient
:Emollient rdf:type owl:Class ;
           rdfs:subClassOf :Ingredient ;
           rdfs:comment "Ingredient of oily nature used in cosmetics to make skin and hair softener. Some of them can serve as solvent for liposoluble actives. Additionally, some of them can act as occlusive ingredients, i.e., they create a barrier to avoid the loss of water. It can be classified according to its chemical nature into the sub-classes:  ester, fatty alcohol, fatty acid, hydrocarbon, silicon, triglyceride."@en ;
           rdfs:label "Emollient"@en .


###  https://purl.org/ontocosmetic#EmollientProperty
:EmollientProperty rdf:type owl:Class ;
                   owl:equivalentClass [ owl:intersectionOf ( :Property
                                                              [ rdf:type owl:Restriction ;
                                                                owl:onProperty :isPropertyOf ;
                                                                owl:hasValue :emollient_type
                                                              ]
                                                            ) ;
                                         rdf:type owl:Class
                                       ] ;
                   rdfs:subClassOf :Property .


###  https://purl.org/ontocosmetic#Emollient_Dosage
:Emollient_Dosage rdf:type owl:Class ;
                  owl:equivalentClass [ owl:intersectionOf ( :Dosage
                                                             [ rdf:type owl:Restriction ;
                                                               owl:onProperty :isQuantifying ;
                                                               owl:someValuesFrom :Emollient
                                                             ]
                                                           ) ;
                                        rdf:type owl:Class
                                      ] ;
                  rdfs:subClassOf :Dosage ;
                  owl:disjointWith :Surfactant_Dosage ;
                  rdfs:comment "Sub-type of dosage which concerns only the emollient."@en ;
                  rdfs:label "Emollient dosage"@en .


###  https://purl.org/ontocosmetic#Emulsion
:Emulsion rdf:type owl:Class ;
          rdfs:subClassOf :Colloid ;
          rdfs:comment "It is a heterogeneous mixture of two or more immiscible liquids. It is a sub-class of a more general class known as colloid."@en .


###  https://purl.org/ontocosmetic#EmulsionScienceHeuristic
:EmulsionScienceHeuristic rdf:type owl:Class ;
                          owl:equivalentClass [ owl:intersectionOf ( :Heuristic
                                                                     [ rdf:type owl:Class ;
                                                                       owl:unionOf ( [ rdf:type owl:Restriction ;
                                                                                       owl:onProperty :hasHeuristicSource ;
                                                                                       owl:hasValue "Heuristic"@en
                                                                                     ]
                                                                                     [ rdf:type owl:Restriction ;
                                                                                       owl:onProperty :hasHeuristicSource ;
                                                                                       owl:hasValue "Heuristic"
                                                                                     ]
                                                                                   )
                                                                     ]
                                                                   ) ;
                                                rdf:type owl:Class
                                              ] ;
                          rdfs:subClassOf :Heuristic ;
                          rdfs:comment "It is a sub-type of heuristic that come from scientific literature."@en .


###  https://purl.org/ontocosmetic#Ester_emollient
:Ester_emollient rdf:type owl:Class ;
                 owl:equivalentClass [ rdf:type owl:Restriction ;
                                       owl:onProperty :hasChemicalNature ;
                                       owl:hasValue :ester
                                     ] ;
                 rdfs:subClassOf :Emollient ;
                 rdfs:comment "chemical compound derived from an oxoacid (organic or inorganic) in which at least one –OH hydroxyl group is replaced by an –O– alkyl (alkoxy) group."@en .


###  https://purl.org/ontocosmetic#Ether_emollient
:Ether_emollient rdf:type owl:Class ;
                 owl:equivalentClass [ rdf:type owl:Restriction ;
                                       owl:onProperty :hasChemicalNature ;
                                       owl:hasValue :ether
                                     ] ;
                 rdfs:subClassOf :Emollient ;
                 rdfs:comment "Sub type of emollient ingredient that are ether."@en .


###  https://purl.org/ontocosmetic#ExpertKnowledgeHeuristic
:ExpertKnowledgeHeuristic rdf:type owl:Class ;
                          owl:equivalentClass [ owl:intersectionOf ( :Heuristic
                                                                     [ rdf:type owl:Restriction ;
                                                                       owl:onProperty :hasHeuristicSource ;
                                                                       owl:hasValue "Matrix"
                                                                     ]
                                                                   ) ;
                                                rdf:type owl:Class
                                              ] ;
                          rdfs:subClassOf :Heuristic ;
                          rdfs:comment "It is a sub-type of heuristic that come from expert  interview."@en .


###  https://purl.org/ontocosmetic#ExtensiveProperty
:ExtensiveProperty rdf:type owl:Class ;
                   rdfs:subClassOf :Property ;
                   rdfs:comment "A measurable characteristic of a substance that depends on the amount of mass of the system (Mass, volume, size)"@en ;
                   rdfs:label "Extensive property"@en .


###  https://purl.org/ontocosmetic#Fatty_alcohol_emollient
:Fatty_alcohol_emollient rdf:type owl:Class ;
                         owl:equivalentClass [ rdf:type owl:Restriction ;
                                               owl:onProperty :hasChemicalNature ;
                                               owl:hasValue :fatty_alcohol
                                             ] ;
                         rdfs:subClassOf :Emollient ;
                         rdfs:comment "Sub type of emollient ingredient that are fatty alcohol."@en .


###  https://purl.org/ontocosmetic#Fluid
:Fluid rdf:type owl:Class ;
       rdfs:subClassOf :StateOfMatter .


###  https://purl.org/ontocosmetic#Foam
:Foam rdf:type owl:Class ;
      rdfs:subClassOf :Colloid ;
      rdfs:comment "gas in liquid."@en .


###  https://purl.org/ontocosmetic#Formulation
:Formulation rdf:type owl:Class ;
             rdfs:subClassOf :Mixture ;
             rdfs:comment "Designed mixture of ingredients combined with an appropriated process. It can potentially take any substance form. It is a technical created object. It can have different forms: solid, liquid, gas. And it can be homogeneous (solutions) or heterogeneous (colloidal system). It is a subclass of substance and a super class of solution, mixture, emulsion, colloid."@en ;
             rdfs:seeAlso :Mixture ,
                          "Blend"@en .


###  https://purl.org/ontocosmetic#FormulationProperty
:FormulationProperty rdf:type owl:Class ;
                     owl:equivalentClass [ owl:intersectionOf ( :Property
                                                                [ rdf:type owl:Restriction ;
                                                                  owl:onProperty :isPropertyOf ;
                                                                  owl:hasValue :formulation_type
                                                                ]
                                                              ) ;
                                           rdf:type owl:Class
                                         ] ;
                     rdfs:subClassOf :Property ;
                     rdfs:comment "Describe the list of properties that a formulated product can have. Formulation heuristic can have an impact on it."@en .


###  https://purl.org/ontocosmetic#FormulationPropertyState
:FormulationPropertyState rdf:type owl:Class ;
                          rdfs:subClassOf :PropertyState .


###  https://purl.org/ontocosmetic#Gel
:Gel rdf:type owl:Class ;
     rdfs:subClassOf :Colloid ;
     rdfs:comment "liquids in solids."@en .


###  https://purl.org/ontocosmetic#Glycols
:Glycols rdf:type owl:Class ;
         rdfs:subClassOf :Humectant ;
         rdfs:comment "They are chemical compounds containing a certain number of hydroxyl groups. They are water- soluble and are widely used in cosmetics due to their moisturizing function. They also work as stabilizer solvents and dispersants of polymers. They have a significant effect on the feel of use."@en .


###  https://purl.org/ontocosmetic#HeterogenousMixture
:HeterogenousMixture rdf:type owl:Class ;
                     rdfs:subClassOf :Mixture ;
                     rdfs:comment "It is a mixture in which the composition is not uniform throughout the mixture. It two or more phases in contact."@en ;
                     rdfs:label "Heterogenous Mixture"@en .


###  https://purl.org/ontocosmetic#Heuristic
:Heuristic rdf:type owl:Class ;
           rdfs:comment "Rules that are used by product formulator to anticipate what happens while combining different ingredients."@en .


###  https://purl.org/ontocosmetic#HeuristicForActive
:HeuristicForActive rdf:type owl:Class ;
                    owl:equivalentClass [ owl:intersectionOf ( :Heuristic
                                                               [ rdf:type owl:Restriction ;
                                                                 owl:onProperty :hasHeuristicIngType ;
                                                                 owl:hasValue :active
                                                               ]
                                                             ) ;
                                          rdf:type owl:Class
                                        ] ;
                    rdfs:subClassOf :Heuristic ;
                    rdfs:comment "Sub group of heuristic that only concerns active ingredients."@en .


###  https://purl.org/ontocosmetic#HeuristicForEmollient
:HeuristicForEmollient rdf:type owl:Class ;
                       rdfs:subClassOf :Heuristic ;
                       rdfs:comment "Sub group of heuristic that only concerns emollients."@en .


###  https://purl.org/ontocosmetic#HeuristicForSurfactant
:HeuristicForSurfactant rdf:type owl:Class ;
                        rdfs:subClassOf :Heuristic ;
                        rdfs:comment "Sub group of heuristic that only concerns surfactants."@en .


###  https://purl.org/ontocosmetic#HeuristicForThickener
:HeuristicForThickener rdf:type owl:Class ;
                       owl:equivalentClass [ owl:intersectionOf ( :Heuristic
                                                                  [ rdf:type owl:Restriction ;
                                                                    owl:onProperty :hasHeuristicIngType ;
                                                                    owl:hasValue :thickener
                                                                  ]
                                                                ) ;
                                             rdf:type owl:Class
                                           ] ;
                       rdfs:subClassOf :Heuristic ;
                       rdfs:comment "Sub group of heuristic that only concerns thickeners."@en .


###  https://purl.org/ontocosmetic#HomogenousMixture
:HomogenousMixture rdf:type owl:Class ;
                   rdfs:subClassOf :Mixture ;
                   rdfs:comment "It is a mixture in which the composition is uniform throughout the mixture. It has only one phase."@en ;
                   rdfs:label "Homogenous Mixture"@en .


###  https://purl.org/ontocosmetic#Humectant
:Humectant rdf:type owl:Class ;
           rdfs:subClassOf :Active ;
           rdfs:comment "Hygroscopic substance used to keep things moist. Most common are glycols."@en .


###  https://purl.org/ontocosmetic#Hydrocarbon_emollient
:Hydrocarbon_emollient rdf:type owl:Class ;
                       owl:equivalentClass [ rdf:type owl:Restriction ;
                                             owl:onProperty :hasChemicalNature ;
                                             owl:hasValue :hydrocarbon
                                           ] ;
                       rdfs:subClassOf :Emollient ;
                       rdfs:comment "Sub type of emollient ingredient that are hydrocarbon."@en .


###  https://purl.org/ontocosmetic#Ingredient
:Ingredient rdf:type owl:Class ;
            rdfs:subClassOf :Substance ;
            rdfs:comment "Substance that forms part of a formulation."@en ;
            rdfs:label "Ingredient"@en .


###  https://purl.org/ontocosmetic#IngredientProperty
:IngredientProperty rdf:type owl:Class ;
                    owl:equivalentClass [ owl:intersectionOf ( :Property
                                                               [ rdf:type owl:Restriction ;
                                                                 owl:onProperty :isPropertyOf ;
                                                                 owl:hasValue :ingredient_type
                                                               ]
                                                             ) ;
                                          rdf:type owl:Class
                                        ] ;
                    rdfs:subClassOf :Property ;
                    rdfs:comment "Describe the properties of the ingredient that is considered by the heuristic. Each instance is a type of property. All the propterties does not concern all the ingredients."@en .


###  https://purl.org/ontocosmetic#IngredientPropertyState
:IngredientPropertyState rdf:type owl:Class ;
                         rdfs:subClassOf :PropertyState .


###  https://purl.org/ontocosmetic#IntensiveProperty
:IntensiveProperty rdf:type owl:Class ;
                   rdfs:subClassOf :Property ;
                   rdfs:comment "A measurable characteristic of a substance that is independent of mass quantity."@en ;
                   rdfs:label "Intensive property"@en .


###  https://purl.org/ontocosmetic#IonicState
:IonicState rdf:type owl:Class ;
            rdfs:subClassOf :IngredientPropertyState .


###  https://purl.org/ontocosmetic#IonicSurfactant
:IonicSurfactant rdf:type owl:Class ;
                 rdfs:subClassOf :Surfactant ;
                 rdfs:label "Ionic surfactant"@en .


###  https://purl.org/ontocosmetic#IonicThickener
:IonicThickener rdf:type owl:Class ;
                rdfs:subClassOf :AqueousThickeners ;
                rdfs:label "Ionic thickener"@en .


###  https://purl.org/ontocosmetic#MicrostructureState
:MicrostructureState rdf:type owl:Class ;
                     rdfs:subClassOf :StructurePropertyState ;
                     rdfs:comment "It is a characteristic of colloidal systems. In this ontology it is described with two phases: Continuous phase and disperse phase."@en .


###  https://purl.org/ontocosmetic#Mixture
:Mixture rdf:type owl:Class ;
         rdfs:subClassOf :Substance ;
         rdfs:comment "It is an entity made up of two or more substances. It can be homogeneous or heterogeneous."@en .


###  https://purl.org/ontocosmetic#NonAqueousThickeners
:NonAqueousThickeners rdf:type owl:Class ;
                      rdfs:subClassOf :Thickener .


###  https://purl.org/ontocosmetic#NonIonicSurfactant
:NonIonicSurfactant rdf:type owl:Class ;
                    rdfs:subClassOf :Surfactant ;
                    rdfs:label "Non ionic surfactant"@en .


###  https://purl.org/ontocosmetic#NonionicThickener
:NonionicThickener rdf:type owl:Class ;
                   rdfs:subClassOf :AqueousThickeners ;
                   rdfs:label "Non ionic thickener"@en .


###  https://purl.org/ontocosmetic#Oiliness
:Oiliness rdf:type owl:Class ;
          rdfs:subClassOf :FormulationPropertyState ;
          rdfs:label "After Feel - Oiliness"@en .


###  https://purl.org/ontocosmetic#OneIngredient
:OneIngredient rdf:type owl:Class ;
               owl:equivalentClass [ rdf:type owl:Restriction ;
                                     owl:onProperty :hasIngredient ;
                                     owl:qualifiedCardinality "1"^^xsd:nonNegativeInteger ;
                                     owl:onClass :Ingredient
                                   ] ;
               rdfs:subClassOf :Mixture .


###  https://purl.org/ontocosmetic#Origin
:Origin rdf:type owl:Class ;
        rdfs:subClassOf :IngredientPropertyState ,
                        :PropertyState ;
        rdfs:comment "It described the origin of the ingredient or product."@en ;
        rdfs:label "Origin type"@en .


###  https://purl.org/ontocosmetic#OtherIngredient
:OtherIngredient rdf:type owl:Class ;
                 rdfs:subClassOf :Ingredient ;
                 rdfs:label "Other ingredient"@en .


###  https://purl.org/ontocosmetic#PhRegulator
:PhRegulator rdf:type owl:Class ;
             rdfs:subClassOf :OtherIngredient ;
             rdfs:label "Ph regulator"@en .


###  https://purl.org/ontocosmetic#PhaseState
:PhaseState rdf:type owl:Class ;
            rdfs:subClassOf :PropertyState .


###  https://purl.org/ontocosmetic#Preservative
:Preservative rdf:type owl:Class ;
              rdfs:subClassOf :OtherIngredient ;
              rdfs:comment "Compounds that prevent products from going off by controlling the growth of microorganisms. Some of them cannot be used for certain product applications and/or they have a maximum allowed concentration in the final product. For their selection, it is important to consider: efficiency, maximal allowed concentration, toxicity, environmental effect, and possible interactions with other emulsion ingredients."@en .


###  https://purl.org/ontocosmetic#Process
:Process rdf:type owl:Class ;
         rdfs:subClassOf :System ;
         rdfs:label "Process"@en .


###  https://purl.org/ontocosmetic#ProcessState
:ProcessState rdf:type owl:Class ;
              rdfs:label "Process state"@en ,
                         "Qualitative value that describes the fomulation processing."@en .


###  https://purl.org/ontocosmetic#Product
:Product rdf:type owl:Class ;
         rdfs:subClassOf :System ;
         rdfs:comment "Formulation ready to go to the market."@en ;
         rdfs:label "Product"@en .


###  https://purl.org/ontocosmetic#ProductProperty
:ProductProperty rdf:type owl:Class ;
                 owl:equivalentClass [ owl:intersectionOf ( :Property
                                                            [ rdf:type owl:Restriction ;
                                                              owl:onProperty :isPropertyOf ;
                                                              owl:hasValue :product_type
                                                            ]
                                                          ) ;
                                       rdf:type owl:Class
                                     ] ;
                 rdfs:subClassOf :Property .


###  https://purl.org/ontocosmetic#Property
:Property rdf:type owl:Class ;
          rdfs:comment "A measurable characteristic related to the physical state or chemical behavior of a substance. They are classified as extensive (depends on the amount of mass of the system) and intensive (independent of mass quantity)."@en ;
          rdfs:seeAlso "physicochemical property"@en .


###  https://purl.org/ontocosmetic#PropertyState
:PropertyState rdf:type owl:Class ;
               rdfs:comment "Define the different qualitative value of properties."@en ;
               rdfs:label "Property state"@en .


###  https://purl.org/ontocosmetic#PureSubstance
:PureSubstance rdf:type owl:Class ;
               rdfs:subClassOf :Substance ;
               rdfs:comment "It is a single kind of substance that cannot be separated into other kinds of substance by any physical means."@en ;
               rdfs:label "Pure Substance"@en .


###  https://purl.org/ontocosmetic#RheologicState
:RheologicState rdf:type owl:Class ;
                rdfs:subClassOf :PropertyState ;
                rdfs:label "Rheologic state"@en .


###  https://purl.org/ontocosmetic#Sensation
:Sensation rdf:type owl:Class ;
           rdfs:subClassOf :FormulationPropertyState ;
           rdfs:comment "Describe the after feel of the formulation on the skin of a consumer. I define the level of oilyness"@en ;
           rdfs:label "After Feel - Absorption Sensation"@en .


###  https://purl.org/ontocosmetic#Silicone_emollient
:Silicone_emollient rdf:type owl:Class ;
                    owl:equivalentClass [ rdf:type owl:Restriction ;
                                          owl:onProperty :hasChemicalNature ;
                                          owl:hasValue :silicone
                                        ] ;
                    rdfs:subClassOf :Emollient ;
                    rdfs:comment "Sub type of emollient ingredient that are silicone."@en .


###  https://purl.org/ontocosmetic#Sol
:Sol rdf:type owl:Class ;
     rdfs:subClassOf :Colloid ;
     rdfs:comment "solid particles in a liquid."@en .


###  https://purl.org/ontocosmetic#SolidFoam
:SolidFoam rdf:type owl:Class ;
           rdfs:subClassOf :Colloid ;
           rdfs:comment "gas in solid."@en .


###  https://purl.org/ontocosmetic#SolidSol
:SolidSol rdf:type owl:Class ;
          rdfs:subClassOf :Colloid ;
          rdfs:comment "solid in solid."@en .


###  https://purl.org/ontocosmetic#Solution
:Solution rdf:type owl:Class ;
          rdfs:subClassOf :HomogenousMixture ;
          rdfs:comment "It is a homogeneous mixture of soluble substances. It does not have a microstructure. It can exist naturally, or it can be technically formulated, and in that case, it can also be named as a Formulation."@en .


###  https://purl.org/ontocosmetic#SpreadingState
:SpreadingState rdf:type owl:Class ;
                rdfs:subClassOf :IngredientPropertyState ;
                rdfs:comment "The ability of the ingredient to spread on the skin"@en .


###  https://purl.org/ontocosmetic#StabilityState
:StabilityState rdf:type owl:Class ;
                rdfs:subClassOf :FormulationPropertyState ;
                rdfs:comment "A formulation can be either stable or note stable."@en .


###  https://purl.org/ontocosmetic#Stabilizer
:Stabilizer rdf:type owl:Class ;
            rdfs:subClassOf :Ingredient ;
            rdfs:comment "Chemical that maintain the function and viscosity of the emulsion. Thus they also act as rheological modifiers. [cosmetic sector definition]"@en .


###  https://purl.org/ontocosmetic#StateOfMatter
:StateOfMatter rdf:type owl:Class ;
               rdfs:subClassOf :PropertyState ;
               rdfs:comment "Substances in formulation design context can have various state: solid, liquid or gaseous."@en ;
               rdfs:label "State of matter"@en .


###  https://purl.org/ontocosmetic#StickinessState
:StickinessState rdf:type owl:Class ;
                 rdfs:subClassOf :FormulationPropertyState ;
                 rdfs:label "After feel - Stickiness"@en .


###  https://purl.org/ontocosmetic#StructurePropertyState
:StructurePropertyState rdf:type owl:Class ;
                        rdfs:subClassOf :PropertyState ;
                        rdfs:comment "Physico-mechanical porpterties of a substance."@en ;
                        rdfs:label "Structure property State"@en .


###  https://purl.org/ontocosmetic#Substance
:Substance rdf:type owl:Class ;
           rdfs:subClassOf :System ;
           rdfs:comment "Any chemical entity (pure and mixture) is a substance."@en ;
           rdfs:label "Substance"@en .


###  https://purl.org/ontocosmetic#SubstanceProperty
:SubstanceProperty rdf:type owl:Class ;
                   rdfs:subClassOf :Property ;
                   rdfs:comment "Chemical properties of a substance."@en ;
                   rdfs:label "Substance property"@en .


###  https://purl.org/ontocosmetic#Surfactant
:Surfactant rdf:type owl:Class ;
            rdfs:subClassOf :Ingredient ;
            rdfs:comment "They are compounds that lower the interfacial tension between two immiscible phases. Surfactants are used in emulsions for four purposes: to decrease the energy required during emulsification, to adsorb rapidly at the interface of recently formed droplets, and to generate a barrier, either electrostatic, steric, or both, for long-term emulsion stability. Additionally, they can be also used as active ingredients in soaps, shampoos and conditioners. They can be classified according to their electrical nature in nonionic, ionic-anionic and ionic-cationic. They can be classified according to their chemical nature."@en ;
            rdfs:seeAlso "emulsifier"@en .


###  https://purl.org/ontocosmetic#SurfactantProperty
:SurfactantProperty rdf:type owl:Class ;
                    owl:equivalentClass [ owl:intersectionOf ( :Property
                                                               [ rdf:type owl:Restriction ;
                                                                 owl:onProperty :isPropertyOf ;
                                                                 owl:hasValue :surfactant_type
                                                               ]
                                                             ) ;
                                          rdf:type owl:Class
                                        ] ;
                    rdfs:subClassOf :Property .


###  https://purl.org/ontocosmetic#Surfactant_Dosage
:Surfactant_Dosage rdf:type owl:Class ;
                   owl:equivalentClass [ owl:intersectionOf ( :Dosage
                                                              [ rdf:type owl:Restriction ;
                                                                owl:onProperty :isQuantifying ;
                                                                owl:someValuesFrom :Surfactant
                                                              ]
                                                            ) ;
                                         rdf:type owl:Class
                                       ] ;
                   rdfs:subClassOf :Dosage ;
                   rdfs:comment "Sub-type of dosage which concerns only the surfactant."@en ;
                   rdfs:label "Surfactant dosage"@en .


###  https://purl.org/ontocosmetic#Suspension
:Suspension rdf:type owl:Class ;
            rdfs:subClassOf :HeterogenousMixture ;
            rdfs:comment "It is cloudy and heterogeneous. The particles are larger than 10,000 Angstroms which allows them to be filtered. If a suspension is allowed to stand the particles will separate out."@en .


###  https://purl.org/ontocosmetic#System
:System rdf:type owl:Class ;
        rdfs:comment "Anything can be described as a system. (Substance, process, product, mixture, etc). It is a superclass of substance and process."@en ;
        rdfs:label "System"@en .


###  https://purl.org/ontocosmetic#TextureState
:TextureState rdf:type owl:Class ;
              rdfs:subClassOf :IngredientPropertyState .


###  https://purl.org/ontocosmetic#Thickener
:Thickener rdf:type owl:Class ;
           rdfs:subClassOf :Ingredient ;
           rdfs:comment "It is a substance that can significantly modify the rheology of a fluid. Rheological modifiers are added to the formulation for three main purposes: to increase viscosity, to promote a particular rheological behavior (pseudo- plastic and thixotropic), and to enhance emulsion stability."@en ;
           rdfs:seeAlso "Rheological modifiers"@en .


###  https://purl.org/ontocosmetic#ThickenerProperty
:ThickenerProperty rdf:type owl:Class ;
                   owl:equivalentClass [ owl:intersectionOf ( :Property
                                                              [ rdf:type owl:Restriction ;
                                                                owl:onProperty :isPropertyOf ;
                                                                owl:hasValue :thickener
                                                              ]
                                                            ) ;
                                         rdf:type owl:Class
                                       ] ;
                   rdfs:subClassOf :Property .


###  https://purl.org/ontocosmetic#UnitOperation
:UnitOperation rdf:type owl:Class ;
               rdfs:comment "Bloc unit of a process."@en ;
               rdfs:label "Unit operation"@en .


###  https://purl.org/ontocosmetic#UvFilter
:UvFilter rdf:type owl:Class ;
          rdfs:subClassOf :Active ;
          rdfs:comment "Ingredients that protect the skin from sun damage and prevent the risks of skin cancer such as melanoma as well as sunburn, premature aging of the skin, or the appearance of spots. They can be mineral (ex. Titanium oxide, zinc oxide) or they can be organic (ex. Octocrylene)."@en .


###  https://purl.org/ontocosmetic#Vegetable_oil_emollient
:Vegetable_oil_emollient rdf:type owl:Class ;
                         owl:equivalentClass [ rdf:type owl:Restriction ;
                                               owl:onProperty :hasChemicalNature ;
                                               owl:hasValue :vegetable_oil
                                             ] ;
                         rdfs:subClassOf :Emollient ;
                         rdfs:comment "Sub type of emollient ingredient that are vegetable oil."@en .


###  https://purl.org/ontocosmetic#ViscosityState
:ViscosityState rdf:type owl:Class ;
                rdfs:subClassOf :PropertyState ;
                rdfs:comment """It is the is a measure of the resistance of a fluid to deformation. It determines the spreadability of the oil and its formulations. Units (mPa*s) 
Describe the level of viscosity of a formulated product. it can be low, medium or high.
It is related to the sensorial term of thickness.""" .


###  https://purl.org/ontocosmetic#anti-age
:anti-age rdf:type owl:Class ;
          rdfs:subClassOf :Active ;
          rdfs:comment "Ingredients that make the consumer look younger by reducing, masking or preventing signs of skin aging."@en .


#################################################################
#    Individuals
#################################################################

###  https://purl.org/ontocosmetic#HLB
:HLB rdf:type owl:NamedIndividual ,
              :Property ;
     :isPropertyOf :surfactant_type ;
     rdfs:label "HLB"@en .


###  https://purl.org/ontocosmetic#HexylLaurate
:HexylLaurate rdf:type owl:NamedIndividual ;
              :hasChemicalNature :ester ;
              :hasSpreading :high_spreading ;
              :hasINCIcode "Hexyl Laurate" ;
              rdfs:label "Hexyl Laurate" .


###  https://purl.org/ontocosmetic#Hexyldecanol
:Hexyldecanol rdf:type owl:NamedIndividual ;
              :hasChemicalNature :fatty_alcohol ;
              :hasOrigin :natural_raw_material ;
              :hasSpreading :medium_spreading ;
              :hasINCIcode "Hexyldecanol" ;
              :hasRequiredHLB "14.0"^^xsd:float ;
              rdfs:label "Hexyldecanol" .


###  https://purl.org/ontocosmetic#HexyldecylStearate
:HexyldecylStearate rdf:type owl:NamedIndividual ;
                    :hasChemicalNature :ester ;
                    :hasSpreading :low_spreading ;
                    :hasINCIcode "Hexyldecyl Stearate" ;
                    rdfs:label "Hexyldecyl Stearate" .


###  https://purl.org/ontocosmetic#NRM_and_SRM
:NRM_and_SRM rdf:type owl:NamedIndividual ,
                      :Origin ;
             rdfs:comment """NRM = Natural Raw Material
SRM = Synthetic Raw Material"""@en .


###  https://purl.org/ontocosmetic#NonStable
:NonStable rdf:type owl:NamedIndividual ,
                    :StabilityState ;
           rdfs:label "Non stable"@en .


###  https://purl.org/ontocosmetic#OilyPhaseConcentration
:OilyPhaseConcentration rdf:type owl:NamedIndividual ,
                                 :StructurePropertyState .


###  https://purl.org/ontocosmetic#Petrolatum
:Petrolatum rdf:type owl:NamedIndividual ;
            :hasChemicalNature :hydrocarbon ;
            :hasINCIcode "Petrolatum" ;
            :hasPricePerKilogram "14.111111"^^xsd:float ;
            rdfs:label "Petrolatum" .


###  https://purl.org/ontocosmetic#Squalane
:Squalane rdf:type owl:NamedIndividual ;
          :hasChemicalNature :hydrocarbon ;
          :hasSpreading :medium_spreading ;
          :hasINCIcode "Squalane" ;
          :hasPricePerKilogram "58.705883"^^xsd:float ;
          rdfs:label "Squalane" .


###  https://purl.org/ontocosmetic#Stable
:Stable rdf:type owl:NamedIndividual ,
                 :StabilityState ;
        rdfs:label "Stable"@en .


###  https://purl.org/ontocosmetic#WaterPhaseConcentration
:WaterPhaseConcentration rdf:type owl:NamedIndividual ,
                                  :StructurePropertyState .


###  https://purl.org/ontocosmetic#absorption_rate
:absorption_rate rdf:type owl:NamedIndividual ,
                          :Property ;
                 rdfs:comment "Describe the capacity of the formulation product to be absopt by a skin."@en ;
                 rdfs:label "Absorption rate"@en .


###  https://purl.org/ontocosmetic#active
:active rdf:type owl:NamedIndividual ,
                 :ChemicalFamily ;
        rdfs:label "Active"@en .


###  https://purl.org/ontocosmetic#after_feeling
:after_feeling rdf:type owl:NamedIndividual ,
                        :Property ;
               :isPropertyOf :ingredient_type ;
               rdfs:label "After feeling"@en .


###  https://purl.org/ontocosmetic#agitation
:agitation rdf:type owl:NamedIndividual ,
                    :UnitOperation .


###  https://purl.org/ontocosmetic#anionic
:anionic rdf:type owl:NamedIndividual ,
                  :IonicState .


###  https://purl.org/ontocosmetic#cloud_point
:cloud_point rdf:type owl:NamedIndividual ,
                      :Property ;
             :isPropertyOf :surfactant_type ;
             rdfs:comment "It corresponds to the temperature at which the surfactant begins to precipitate when the temperature is increased. Emulsions are destabilized above this temperature (maximal temperature for stability)."@en ;
             rdfs:label "Cloud point"@en .


###  https://purl.org/ontocosmetic#complete_sensoriel_profile
:complete_sensoriel_profile rdf:type owl:NamedIndividual ,
                                     :Sensation ;
                            rdfs:label "Complete sensoriel profile"@en .


###  https://purl.org/ontocosmetic#cooling
:cooling rdf:type owl:NamedIndividual ,
                  :UnitOperation .


###  https://purl.org/ontocosmetic#cream
:cream rdf:type owl:NamedIndividual ,
                :TextureState ;
       rdfs:label "Cream"@en .


###  https://purl.org/ontocosmetic#critical_micelle_concentration
:critical_micelle_concentration rdf:type owl:NamedIndividual ,
                                         :Property ;
                                :isPropertyOf :surfactant_type ;
                                rdfs:comment "It is the concentration at which the surfactant molecules begin to form micelles in an aqueous solution, i.e., an aggregate structure of surfactant molecules. Below CMC, surface tension is reduced when the surfactant concentration increases; above CMC, the surface tension remains constant."@en ;
                                rdfs:label "Critical micelle concentration"@en .


###  https://purl.org/ontocosmetic#density
:density rdf:type owl:NamedIndividual ,
                  :Property ;
         rdfs:comment "It is the mass per unit of volume. In emulsions it is related to emulsion stability."@en ;
         rdfs:label "Density"@en .


###  https://purl.org/ontocosmetic#droplet_size
:droplet_size rdf:type owl:NamedIndividual ,
                       :StructurePropertyState ;
              rdfs:comment "Fromulated product can be emulsions. These emulsions are caracterized by the size of the droplets."@en ;
              rdfs:label "Droplet size"@en .


###  https://purl.org/ontocosmetic#efficiency
:efficiency rdf:type owl:NamedIndividual ,
                     :Property ;
            :isPropertyOf :thickener ;
            rdfs:comment "It is the ability to increase viscosity using a certain quantity of the rheological modifier. Efficiency depends on the polymer nature, molecular weight, branches, and conformation."@en ;
            rdfs:label "Efficiency"@en .


###  https://purl.org/ontocosmetic#electrical_nature
:electrical_nature rdf:type owl:NamedIndividual ,
                            :Property ;
                   :isPropertyOf :surfactant_type ;
                   rdfs:label "Electrical nature"@en .


###  https://purl.org/ontocosmetic#emollient_type
:emollient_type rdf:type owl:NamedIndividual ,
                         :ChemicalFamily ;
                rdfs:label "Emollient type"@en .


###  https://purl.org/ontocosmetic#ester
:ester rdf:type owl:NamedIndividual ,
                :Chemical_nature ;
       rdfs:label "Ester"@en .


###  https://purl.org/ontocosmetic#ether
:ether rdf:type owl:NamedIndividual ,
                :Chemical_nature ;
       rdfs:label "Ether"@en .


###  https://purl.org/ontocosmetic#fatty_acid
:fatty_acid rdf:type owl:NamedIndividual ,
                     :Chemical_nature ;
            rdfs:comment "Category of emollient that are carboxylic acid with an aliphatic chain."@en ;
            rdfs:label "Fatty acid"@en .


###  https://purl.org/ontocosmetic#fatty_alcohol
:fatty_alcohol rdf:type owl:NamedIndividual ,
                        :Chemical_nature ;
               rdfs:comment "Category of emollients that are usually high-molecular-weight derived from natural fats and oils."@en ;
               rdfs:label "fatty alcohol"@en .


###  https://purl.org/ontocosmetic#formulation_type
:formulation_type rdf:type owl:NamedIndividual ,
                           :ChemicalFamily ;
                  rdfs:label "Formulation type"@en .


###  https://purl.org/ontocosmetic#gas
:gas rdf:type owl:NamedIndividual ,
              :Fluid ,
              :StateOfMatter ;
     rdfs:comment "State of matter. It is a substance in a state that takes the shape and volume of its container."@en ;
     rdfs:label "Gas"@en .


###  https://purl.org/ontocosmetic#gel
:gel rdf:type owl:NamedIndividual ,
              :TextureState ;
     rdfs:label "Gel"@en .


###  https://purl.org/ontocosmetic#heating
:heating rdf:type owl:NamedIndividual ,
                  :UnitOperation .


###  https://purl.org/ontocosmetic#high_absorption_rate
:high_absorption_rate rdf:type owl:NamedIndividual ,
                               :AbsorptionRateState ;
                      rdfs:label "High absorption rate"@en .


###  https://purl.org/ontocosmetic#high_agitation
:high_agitation rdf:type owl:NamedIndividual ,
                         :AgitationState ;
                rdfs:label "High agitation"@en .


###  https://purl.org/ontocosmetic#high_droplet
:high_droplet rdf:type owl:NamedIndividual ,
                       :DropletSizeState ;
              rdfs:label "High droplet"@en .


###  https://purl.org/ontocosmetic#high_spreading
:high_spreading rdf:type owl:NamedIndividual ,
                         :SpreadingState ;
                rdfs:label "High spreading"@en .


###  https://purl.org/ontocosmetic#high_viscosity
:high_viscosity rdf:type owl:NamedIndividual ,
                         :ViscosityState ;
                rdfs:label "High viscosity"@en .


###  https://purl.org/ontocosmetic#homogenous
:homogenous rdf:type owl:NamedIndividual ,
                     :MicrostructureState .


###  https://purl.org/ontocosmetic#hydrocarbon
:hydrocarbon rdf:type owl:NamedIndividual ,
                      :Chemical_nature ;
             rdfs:comment "Catergory of emmolients that have organic compound consisting entirely of hydrogen and carbon."@en ;
             rdfs:label "Hydrocarbon"@en .


###  https://purl.org/ontocosmetic#incomplete_sensoriel_profile
:incomplete_sensoriel_profile rdf:type owl:NamedIndividual ,
                                       :Sensation ;
                              rdfs:label "Incomplete sensorial profile"@en .


###  https://purl.org/ontocosmetic#ingredient_type
:ingredient_type rdf:type owl:NamedIndividual ,
                          :ChemicalFamily ;
                 rdfs:label "Ingredient type"@en .


###  https://purl.org/ontocosmetic#kraft_point
:kraft_point rdf:type owl:NamedIndividual ,
                      :Property ;
             :isPropertyOf :surfactant_type ;
             rdfs:comment "It is the minimal temperature at which surfactants begin to form micelles. Below this temperature, the solubility of surfactant is low. Stable emulsions are only formed above this temperature (minimal temperature for stability)."@en ;
             rdfs:label "Kraft point"@en .


###  https://purl.org/ontocosmetic#light_emollience
:light_emollience rdf:type owl:NamedIndividual ,
                           :EmollienceState ;
                  rdfs:label "Light emollience"@en .


###  https://purl.org/ontocosmetic#liquid
:liquid rdf:type owl:NamedIndividual ,
                 :Fluid ,
                 :StateOfMatter ;
        rdfs:comment "State of matter. It is a substance in a state that takes the shape of its container but retains a (nearly) constant volume independent of pressure"@en ;
        rdfs:label "Liquid"@en .


###  https://purl.org/ontocosmetic#lotion
:lotion rdf:type owl:NamedIndividual ,
                 :TextureState ;
        rdfs:label "Lotion"@en .


###  https://purl.org/ontocosmetic#low_absorption_rate
:low_absorption_rate rdf:type owl:NamedIndividual ,
                              :AbsorptionRateState ;
                     rdfs:label "Low absorption rate"@en .


###  https://purl.org/ontocosmetic#low_agitation
:low_agitation rdf:type owl:NamedIndividual ,
                        :AgitationState ;
               rdfs:label "Low agitation"@en .


###  https://purl.org/ontocosmetic#low_spreading
:low_spreading rdf:type owl:NamedIndividual ,
                        :SpreadingState ;
               rdfs:label "Low spreading"@en .


###  https://purl.org/ontocosmetic#low_viscosity
:low_viscosity rdf:type owl:NamedIndividual ,
                        :ViscosityState ;
               rdfs:label "Low viscosity"@en .


###  https://purl.org/ontocosmetic#med_absorption_rate
:med_absorption_rate rdf:type owl:NamedIndividual ,
                              :AbsorptionRateState ;
                     rdfs:label "Medium absorption rate"@en .


###  https://purl.org/ontocosmetic#med_agitation
:med_agitation rdf:type owl:NamedIndividual ,
                        :AgitationState ;
               rdfs:label "Medium agitation"@en .


###  https://purl.org/ontocosmetic#med_droplet
:med_droplet rdf:type owl:NamedIndividual ,
                      :DropletSizeState ;
             rdfs:label "Medium droplet"@en .


###  https://purl.org/ontocosmetic#med_viscosity
:med_viscosity rdf:type owl:NamedIndividual ,
                        :ViscosityState ;
               rdfs:label "Medium viscosity"@en .


###  https://purl.org/ontocosmetic#medium_emollience
:medium_emollience rdf:type owl:NamedIndividual ,
                            :EmollienceState ;
                   rdfs:label "Medium emollience"@en .


###  https://purl.org/ontocosmetic#medium_spreading
:medium_spreading rdf:type owl:NamedIndividual ,
                           :SpreadingState ;
                  rdfs:label "Medium spreading"@en .


###  https://purl.org/ontocosmetic#medium_to_high_spreading
:medium_to_high_spreading rdf:type owl:NamedIndividual ,
                                   :SpreadingState ;
                          rdfs:label "Medium to high spreading"@en .


###  https://purl.org/ontocosmetic#medium_to_light_emollience
:medium_to_light_emollience rdf:type owl:NamedIndividual ,
                                     :EmollienceState ;
                            rdfs:label "Medium to light emollience"@en .


###  https://purl.org/ontocosmetic#medium_to_low_spreading
:medium_to_low_spreading rdf:type owl:NamedIndividual ,
                                  :SpreadingState ;
                         rdfs:label "Medium to low psreading"@en .


###  https://purl.org/ontocosmetic#medium_to_rich_emollience
:medium_to_rich_emollience rdf:type owl:NamedIndividual ,
                                    :EmollienceState ;
                           rdfs:label "Medium to rich emollience"@en .


###  https://purl.org/ontocosmetic#melting_point
:melting_point rdf:type owl:NamedIndividual ,
                        :Property ;
               rdfs:comment "It is the temperature in which a substance in the solid-state melts and change to a liquid state. It is important for the selection of ingredients and process conditions. For example, in the case of emollients, it determines if the emollient is solid or liquid, its consistency, and the possible consistency of the resulting formulation."@en ;
               rdfs:label "Melting point"@en .


###  https://purl.org/ontocosmetic#microstructure
:microstructure rdf:type owl:NamedIndividual ,
                         :StructurePropertyState ;
                rdfs:label "Microstructure"@en .


###  https://purl.org/ontocosmetic#natural
:natural rdf:type owl:NamedIndividual ,
                  :Origin .


###  https://purl.org/ontocosmetic#natural_and_SRM
:natural_and_SRM rdf:type owl:NamedIndividual ,
                          :Origin .


###  https://purl.org/ontocosmetic#natural_raw_material
:natural_raw_material rdf:type owl:NamedIndividual ,
                               :Origin .


###  https://purl.org/ontocosmetic#natural_raw_material_enzymatic_processed
:natural_raw_material_enzymatic_processed rdf:type owl:NamedIndividual ,
                                                   :Origin .


###  https://purl.org/ontocosmetic#no_sticky_sensation
:no_sticky_sensation rdf:type owl:NamedIndividual ,
                              :StickinessState ;
                     rdfs:label "No sticky sensation"@en .


###  https://purl.org/ontocosmetic#non-organic
:non-organic rdf:type owl:NamedIndividual ,
                      :Chemical_nature .


###  https://purl.org/ontocosmetic#non_oily
:non_oily rdf:type owl:NamedIndividual ,
                   :Oiliness ;
          rdfs:label "Non oily"@en .


###  https://purl.org/ontocosmetic#nonionic
:nonionic rdf:type owl:NamedIndividual ,
                   :IonicState .


###  https://purl.org/ontocosmetic#oil-in-water
:oil-in-water rdf:type owl:NamedIndividual ,
                       :MicrostructureState ;
              rdfs:label "Oil in water"@en .


###  https://purl.org/ontocosmetic#oiliness
:oiliness rdf:type owl:NamedIndividual ,
                   :Property ;
          :isPropertyOf :formulation_type ;
          rdfs:label "Oiliness"@en .


###  https://purl.org/ontocosmetic#oily
:oily rdf:type owl:NamedIndividual ,
               :Oiliness ;
      rdfs:label "Oily"@en .


###  https://purl.org/ontocosmetic#oily_phase
:oily_phase rdf:type owl:NamedIndividual ,
                     :PhaseState ;
            rdfs:label "Oily phase"@en .


###  https://purl.org/ontocosmetic#phase
:phase rdf:type owl:NamedIndividual ,
                :Property ;
       :isPropertyOf :ingredient_type ;
       rdfs:comment "It is a region of space throughout which all physical properties of a material are essentially uniform."@en ;
       rdfs:label "Phase"@en .


###  https://purl.org/ontocosmetic#polarity
:polarity rdf:type owl:NamedIndividual ,
                   :Property ;
          rdfs:comment "It is a property that represent the separation of the electrical charge within the same molecule. The polarity determines the types of inter-molecular forces of the substance. Thus, it is related to other properties such as solubility, boiling point, fusion point, among others."@en ;
          rdfs:label "Polarity"@en .


###  https://purl.org/ontocosmetic#product_type
:product_type rdf:type owl:NamedIndividual ,
                       :ChemicalFamily ;
              rdfs:label "Product type"@en .


###  https://purl.org/ontocosmetic#pseudoplastic
:pseudoplastic rdf:type owl:NamedIndividual ,
                        :RheologicState .


###  https://purl.org/ontocosmetic#recommanded_usage
:recommanded_usage rdf:type owl:NamedIndividual ,
                            :Property ;
                   :isPropertyOf :ingredient_type ;
                   rdfs:label "Recommanded usage"@en .


###  https://purl.org/ontocosmetic#required_hlb
:required_hlb rdf:type owl:NamedIndividual ,
                       :Property ;
              rdfs:comment """It represents the HLB needed by an oil or a mixture of oils to be more likely to be incorporated in a stable O/W emulsion by an emulsifier or blend of emulsifiers. It determines the compatibility of oils with the surfactant system.
The value of the required HLB of an emollient blend corresponds to the average of the HLB required by each emollient weighted by its mass composition in the emollient mixture."""@en ;
              rdfs:label "Required HLB"@en .


###  https://purl.org/ontocosmetic#rheology
:rheology rdf:type owl:NamedIndividual ,
                   :Property ;
          :isPropertyOf :ingredient_type ;
          rdfs:label "Rheology"@en .


###  https://purl.org/ontocosmetic#rich_emollience
:rich_emollience rdf:type owl:NamedIndividual ,
                          :EmollienceState ;
                 rdfs:label "Rich emollience"@en .


###  https://purl.org/ontocosmetic#sensorial_profile
:sensorial_profile rdf:type owl:NamedIndividual ,
                            :Property ;
                   rdfs:label "Sensorial profile"@en .


###  https://purl.org/ontocosmetic#silicone
:silicone rdf:type owl:NamedIndividual ,
                   :Chemical_nature ;
          rdfs:comment "Category of emollient that are polysiloxane which is a polymer made up of siloxane (−R2Si−O−SiR2−)"@en .


###  https://purl.org/ontocosmetic#silky
:silky rdf:type owl:NamedIndividual ,
                :AfterfeelingState .


###  https://purl.org/ontocosmetic#small_droplet
:small_droplet rdf:type owl:NamedIndividual ,
                        :DropletSizeState ;
               rdfs:label "Small droplet"@en .


###  https://purl.org/ontocosmetic#smooth
:smooth rdf:type owl:NamedIndividual ,
                 :AfterfeelingState .


###  https://purl.org/ontocosmetic#solid
:solid rdf:type owl:NamedIndividual ,
                :StateOfMatter ;
       rdfs:comment "State of matter. It has an structural rigidity and a resistance to a force applied to the surface."@en ;
       rdfs:label "Solid"@en .


###  https://purl.org/ontocosmetic#solubility_in_water
:solubility_in_water rdf:type owl:NamedIndividual ,
                              :Property ;
                     :isPropertyOf :thickener ;
                     rdfs:label "Solubility in water"@en .


###  https://purl.org/ontocosmetic#source
:source rdf:type owl:NamedIndividual ,
                 :Property ;
        :isPropertyOf :ingredient_type ,
                      :product_type ;
        rdfs:label "Source"@en .


###  https://purl.org/ontocosmetic#special_function
:special_function rdf:type owl:NamedIndividual ,
                           :Property ;
                  :isPropertyOf :formulation_type ;
                  rdfs:label "Special function"@en .


###  https://purl.org/ontocosmetic#spray
:spray rdf:type owl:NamedIndividual ,
                :TextureState .


###  https://purl.org/ontocosmetic#spreading
:spreading rdf:type owl:NamedIndividual ,
                    :Property ;
           :isPropertyOf :ingredient_type ;
           rdfs:label "Spreading"@en .


###  https://purl.org/ontocosmetic#stability
:stability rdf:type owl:NamedIndividual ,
                    :Property ;
           :isPropertyOf :formulation_type ;
           rdfs:comment "A formulation can be either stable or note stable."@en ;
           rdfs:label "Stability"@en .


###  https://purl.org/ontocosmetic#stickiness
:stickiness rdf:type owl:NamedIndividual ,
                     :Property ;
            :isPropertyOf :formulation_type ;
            rdfs:label "Stickiness"@en .


###  https://purl.org/ontocosmetic#sticky_sensation
:sticky_sensation rdf:type owl:NamedIndividual ,
                           :StickinessState ;
                  rdfs:label "Sticky sensation"@en .


###  https://purl.org/ontocosmetic#surfactant_type
:surfactant_type rdf:type owl:NamedIndividual ,
                          :ChemicalFamily ;
                 rdfs:label "Surfactant type"@en .


###  https://purl.org/ontocosmetic#synthetic
:synthetic rdf:type owl:NamedIndividual ,
                    :Origin .


###  https://purl.org/ontocosmetic#texture
:texture rdf:type owl:NamedIndividual ,
                  :Property ;
         :isPropertyOf :ingredient_type ;
         rdfs:label "Texture"@en .


###  https://purl.org/ontocosmetic#thickener
:thickener rdf:type owl:NamedIndividual ,
                    :ChemicalFamily ;
           rdfs:label "Thickener type"@en .


###  https://purl.org/ontocosmetic#thickener_stability
:thickener_stability rdf:type owl:NamedIndividual ,
                              :Property ;
                     :isPropertyOf :thickener ;
                     rdfs:comment "Stability with other ingredients because some rheological modifiers may cause the precipitation of other ingredients in the formula."@en ;
                     rdfs:label "Thickener stability"@en .


###  https://purl.org/ontocosmetic#thixotropic
:thixotropic rdf:type owl:NamedIndividual ,
                      :RheologicState .


###  https://purl.org/ontocosmetic#transport_and_release
:transport_and_release rdf:type owl:NamedIndividual ,
                                :Property ;
                       :isPropertyOf :formulation_type ;
                       rdfs:label "Transport and realease"@en .


###  https://purl.org/ontocosmetic#triglyceride
:triglyceride rdf:type owl:NamedIndividual ,
                       :Chemical_nature ;
              rdfs:comment "Category of emollients that are ester derived from glycerol and three fatty acids"@en .


###  https://purl.org/ontocosmetic#vegetable_oil
:vegetable_oil rdf:type owl:NamedIndividual ,
                        :Chemical_nature .


###  https://purl.org/ontocosmetic#vegetable_wax
:vegetable_wax rdf:type owl:NamedIndividual ,
                        :Chemical_nature .


###  https://purl.org/ontocosmetic#very_high_spreading
:very_high_spreading rdf:type owl:NamedIndividual ,
                              :SpreadingState .


###  https://purl.org/ontocosmetic#very_oily
:very_oily rdf:type owl:NamedIndividual ,
                    :Oiliness ;
           rdfs:comment "Very high oily sensation provided by a formulation. It is a value of the oiliness property."@en ;
           rdfs:label "Very oily"@en .


###  https://purl.org/ontocosmetic#very_waterly
:very_waterly rdf:type owl:NamedIndividual ,
                       :Oiliness ;
              rdfs:label "Very waterly"@en .


###  https://purl.org/ontocosmetic#viscosity
:viscosity rdf:type owl:NamedIndividual ,
                    :Property ;
           rdfs:comment """It is the is a measure of the resistance of a fluid to deformation. It determines the spreadability of the oil and its formulations. Units (mPa*s) 
Describe the level of viscosity of a formulated product. it can be low, medium or high.
It is related to the sensorial term of thickness."""@en ;
           rdfs:label "Viscosity"@en .


###  https://purl.org/ontocosmetic#visual_appearance
:visual_appearance rdf:type owl:NamedIndividual ,
                            :Property ;
                   :isPropertyOf :formulation_type ;
                   rdfs:comment "Property that describes the color and transparency."@en ;
                   rdfs:label "Visual appearance"@en .


###  https://purl.org/ontocosmetic#water-in-oil
:water-in-oil rdf:type owl:NamedIndividual ,
                       :MicrostructureState ;
              rdfs:label "Water in oil"@en .


###  https://purl.org/ontocosmetic#water_phase
:water_phase rdf:type owl:NamedIndividual ,
                      :PhaseState ;
             rdfs:label "Water phase"@en .


###  https://purl.org/ontocosmetic#waterly
:waterly rdf:type owl:NamedIndividual ,
                  :Oiliness ;
         rdfs:comment "Water sensation provided by a formulation. It is a value of the oiliness property."@en ;
         rdfs:label "Waterly"@en .


###  https://purl.org/ontocosmetic#waxy
:waxy rdf:type owl:NamedIndividual ,
               :AfterfeelingState .


###  https://purl.org/ontocosmetic#HelianthusAnnuus(sunflowerseed)Oil
<https://purl.org/ontocosmetic#HelianthusAnnuus(sunflowerseed)Oil> rdf:type owl:NamedIndividual ;
                                                                   :hasChemicalNature :vegetable_oil ;
                                                                   :hasOrigin :natural_raw_material ;
                                                                   :hasSpreading :low_spreading ;
                                                                   :hasINCIcode "Helianthus Annuus (sunflower seed) oil" ;
                                                                   :hasPricePerKilogram "12.166667"^^xsd:float ;
                                                                   :hasRequiredHLB "6.0"^^xsd:float ;
                                                                   rdfs:label "Helianthus Annuus (sunflower seed) oil" .


###  https://purl.org/ontocosmetic#TheobromaCacao(Cocoabutter)
<https://purl.org/ontocosmetic#TheobromaCacao(Cocoabutter)> rdf:type owl:NamedIndividual ;
                                                            :hasChemicalNature :vegetable_oil ;
                                                            :hasOrigin :natural_raw_material ;
                                                            :hasINCIcode "Theobroma cacao (Cocoa butter)" ;
                                                            :hasPricePerKilogram "20.2"^^xsd:float ;
                                                            :hasRequiredHLB "6.0"^^xsd:float ;
                                                            rdfs:label "Theobroma cacao (Cocoa butter)" .


#################################################################
#    General axioms
#################################################################

[ rdf:type owl:AllDisjointClasses ;
  owl:members ( :AfterfeelingState
                :Chemical_nature
                :Dosage
                :EmollienceState
                :Formulation
                :Heuristic
                :Ingredient
                :IonicState
                :Origin
                :SpreadingState
                :TextureState
              )
] .


[ rdf:type owl:AllDisjointClasses ;
  owl:members ( :HeterogenousMixture
                :HomogenousMixture
                :OneIngredient
              )
] .


[ rdf:type owl:AllDifferent ;
  owl:distinctMembers ( :NonStable
                        :Stable
                      )
] .


[ rdf:type owl:AllDifferent ;
  owl:distinctMembers ( :gas
                        :liquid
                      )
] .


[ rdf:type owl:AllDifferent ;
  owl:distinctMembers ( :gas
                        :solid
                      )
] .


[ rdf:type owl:AllDifferent ;
  owl:distinctMembers ( :high_absorption_rate
                        :low_absorption_rate
                      )
] .


[ rdf:type owl:AllDifferent ;
  owl:distinctMembers ( :high_absorption_rate
                        :med_absorption_rate
                      )
] .


[ rdf:type owl:AllDifferent ;
  owl:distinctMembers ( :high_agitation
                        :low_agitation
                      )
] .


[ rdf:type owl:AllDifferent ;
  owl:distinctMembers ( :high_agitation
                        :med_agitation
                      )
] .


[ rdf:type owl:AllDifferent ;
  owl:distinctMembers ( :high_droplet
                        :med_droplet
                      )
] .


[ rdf:type owl:AllDifferent ;
  owl:distinctMembers ( :high_droplet
                        :small_droplet
                      )
] .


[ rdf:type owl:AllDifferent ;
  owl:distinctMembers ( :high_spreading
                        :low_spreading
                      )
] .


[ rdf:type owl:AllDifferent ;
  owl:distinctMembers ( :high_spreading
                        :medium_spreading
                      )
] .


[ rdf:type owl:AllDifferent ;
  owl:distinctMembers ( :high_viscosity
                        :low_viscosity
                        :med_viscosity
                      )
] .


[ rdf:type owl:AllDifferent ;
  owl:distinctMembers ( :light_emollience
                        :medium_emollience
                      )
] .


[ rdf:type owl:AllDifferent ;
  owl:distinctMembers ( :light_emollience
                        :rich_emollience
                      )
] .


[ rdf:type owl:AllDifferent ;
  owl:distinctMembers ( :liquid
                        :solid
                      )
] .


[ rdf:type owl:AllDifferent ;
  owl:distinctMembers ( :low_absorption_rate
                        :med_absorption_rate
                      )
] .


[ rdf:type owl:AllDifferent ;
  owl:distinctMembers ( :low_agitation
                        :med_agitation
                      )
] .


[ rdf:type owl:AllDifferent ;
  owl:distinctMembers ( :low_spreading
                        :medium_spreading
                      )
] .


[ rdf:type owl:AllDifferent ;
  owl:distinctMembers ( :medium_emollience
                        :rich_emollience
                      )
] .


[ rdf:type owl:AllDifferent ;
  owl:distinctMembers ( :medium_to_light_emollience
                        :rich_emollience
                      )
] .


[ rdf:type owl:AllDifferent ;
  owl:distinctMembers ( :medium_to_rich_emollience
                        :rich_emollience
                      )
] .


[ rdf:type owl:AllDifferent ;
  owl:distinctMembers ( :non_oily
                        :oily
                      )
] .


[ rdf:type owl:AllDifferent ;
  owl:distinctMembers ( :non_oily
                        :very_oily
                      )
] .


[ rdf:type owl:AllDifferent ;
  owl:distinctMembers ( :non_oily
                        :very_waterly
                      )
] .


[ rdf:type owl:AllDifferent ;
  owl:distinctMembers ( :non_oily
                        :waterly
                      )
] .


[ rdf:type owl:AllDifferent ;
  owl:distinctMembers ( :oily
                        :very_waterly
                      )
] .


[ rdf:type owl:AllDifferent ;
  owl:distinctMembers ( :oily_phase
                        :water_phase
                      )
] .


[ rdf:type owl:AllDifferent ;
  owl:distinctMembers ( :very_oily
                        :very_waterly
                      )
] .


[ rdf:type owl:AllDifferent ;
  owl:distinctMembers ( :very_oily
                        :waterly
                      )
] .


[ rdf:type owl:AllDifferent ;
  owl:distinctMembers ( :very_waterly
                        :waterly
                      )
] .


###  Generated by the OWL API (version 5.1.18) https://github.com/owlcs/owlapi/
